Cleaner measures

ReducibilityMeasure.v
@@ -14,10 +14,10 @@ Require Import Coq.Program.Program.
 
 Require Import Omega.
 
-Definition index (T: tree): option tree :=
+Definition index (T: tree): tree :=
   match T with
-  | T_rec n _ _ => Some n
-  | _ => None
+  | T_rec n _ _ => n
+  | _ => notype_err
   end.
 
 Set Program Mode.
@@ -50,14 +50,11 @@ Proof.
   induction v; repeat step || step_inversion is_nat_value.
 Qed.
 
-Definition lt_index (i1 i2: option tree) :=
-  (exists n, i1 = Some n /\ i2 = None) \/
-  (exists n1 n2 v1 v2 (p1: is_nat_value v1) (p2: is_nat_value v2),
-     i1 = Some n1 /\
-     i2 = Some n2 /\
-     star small_step n1 v1 /\
-     star small_step n2 v2 /\
-     nat_value_to_nat v1 p1 < nat_value_to_nat v2 p2)
+Definition lt_index (t1 t2: tree) :=
+  exists v1 v2 (p1: is_nat_value v1) (p2: is_nat_value v2),
+     star small_step t1 v1 /\
+     star small_step t2 v2 /\
+     nat_value_to_nat v1 p1 < nat_value_to_nat v2 p2
 .
 
 Ltac tlu :=
@@ -65,11 +62,11 @@ Ltac tlu :=
   | H: lt_index _ _ |- _ => unfold lt_index in H
   end.
 
-Lemma acc_ind:
-  forall m n v (p: is_nat_value v),
+Lemma acc_ind_aux:
+  forall m t v (p: is_nat_value v),
     nat_value_to_nat v p < m ->
-    star small_step n v ->
-    Acc lt_index (Some n).
+    star small_step t v ->
+    Acc lt_index t.
 Proof.
   induction m; destruct p; steps; try omega.
   - apply Acc_intro; repeat step || tlu || t_deterministic_star || simp nat_value_to_nat in *; try omega.
@@ -82,30 +79,24 @@ Proof.
     end; eauto with omega.
 Qed.
 
-Lemma acc_ind_some:
-  forall n, Acc lt_index (Some n).
+Lemma acc_ind:
+  forall n, Acc lt_index n.
 Proof.
-  intro; apply Acc_intro; repeat step || tlu; eauto using acc_ind.
-Qed.
-
-Lemma acc_ind_none:
-  Acc lt_index None.
-Proof.
-  apply Acc_intro; repeat step || tlu; eauto using acc_ind_some.
+  intro; apply Acc_intro; repeat step || tlu; eauto using acc_ind_aux.
 Qed.
 
 Lemma wf_lt_index: well_founded lt_index.
 Proof.
   unfold well_founded.
-  destruct a; repeat step; eauto using acc_ind_some, acc_ind_none.
+  destruct a; repeat step; eauto using acc_ind.
 Qed.
 
 Instance wellfounded_lt_index :
   WellFounded lt_index := wf_lt_index.
 
-Notation "p1 '<<' p2" := (lexprod nat (option tree) lt lt_index p1 p2) (at level 80).
+Notation "p1 '<<' p2" := (lexprod nat tree lt lt_index p1 p2) (at level 80).
 
-Definition wf_measure := wellfounded_lexprod nat (option tree) lt lt_index lt_wf wf_lt_index.
+Definition wf_measure := wellfounded_lexprod nat tree lt lt_index lt_wf wf_lt_index.
 
 Opaque lt.
 
@@ -117,12 +108,6 @@ Proof.
   repeat step.
   pose proof (wf_measure (a,b)).
   induction H; steps.
-Qed.
-
-Lemma lt_index_some_none:
-  forall i, lt_index (Some i) None.
-Proof.
-  unfold lt_index; steps; eauto.
 Qed.
 
 Lemma nat_value_to_nat_succ:
@@ -140,10 +125,10 @@ Lemma lt_index_step:
   forall t v,
     star small_step t (succ v) ->
     is_nat_value v ->
-    lt_index (Some v) (Some t).
+    lt_index v t.
 Proof.
-  unfold lt_index; right.
-  unshelve eexists v, t, v, (succ v), _, _; steps;
+  unfold lt_index; intros.
+  unshelve eexists v, (succ v), _, _; steps;
     eauto with b_inv;
     eauto using nat_value_to_nat_succ.
 Qed.
